pkvm_handler/a7424.v
@@ -22,13 +22,13 @@ Definition a7424 : isla_trace :=
   Smt (DefineConst 43%Z (Manyop (Bvmanyarith Bvadd) [Val (Val_Symbolic 29%Z) Mk_annot; Val (Val_Bits (BV 64%N 0x3d4%Z)) Mk_annot] Mk_annot)) Mk_annot :t:
   Smt (DefineConst 70%Z (Binop (Eq) (Val (Val_Symbolic 43%Z) Mk_annot) (Manyop (Bvmanyarith Bvand) [Val (Val_Symbolic 43%Z) Mk_annot; Val (Val_Bits (BV 64%N 0xfffffffffffffff8%Z)) Mk_annot] Mk_annot) Mk_annot)) Mk_annot :t:
   ReadReg "PSTATE" [Field "D"] (RegVal_Struct [("D", RegVal_Base (Val_Symbolic 6%Z))]) Mk_annot :t:
-  Smt (DeclareConst 2281%Z (Ty_BitVec 56%N)) Mk_annot :t:
-  Smt (DefineConst 2290%Z (Unop (ZeroExtend 8%N) (Manyop Concat [Val (Val_Bits (BV 4%N 0x0%Z)) Mk_annot; Unop (Extract 51%N 0%N) (Val (Val_Symbolic 43%Z) Mk_annot) Mk_annot] Mk_annot) Mk_annot)) Mk_annot :t:
-  Smt (DeclareConst 2291%Z (Ty_BitVec 64%N)) Mk_annot :t:
-  ReadMem (RegVal_Base (Val_Symbolic 2291%Z)) (RegVal_Base (Val_Enum ((Mk_enum_id 6%nat), Mk_enum_ctor 0%nat))) (RegVal_Base (Val_Symbolic 2290%Z)) 8%N None Mk_annot :t:
-  Smt (DefineConst 2294%Z (Val (Val_Symbolic 2291%Z) Mk_annot)) Mk_annot :t:
-  WriteReg "R5" [] (RegVal_Base (Val_Symbolic 2294%Z)) Mk_annot :t:
-  Smt (DefineConst 2295%Z (Manyop (Bvmanyarith Bvadd) [Val (Val_Symbolic 29%Z) Mk_annot; Val (Val_Bits (BV 64%N 0x4%Z)) Mk_annot] Mk_annot)) Mk_annot :t:
-  WriteReg "_PC" [] (RegVal_Base (Val_Symbolic 2295%Z)) Mk_annot :t:
+  Smt (DeclareConst 1311%Z (Ty_BitVec 56%N)) Mk_annot :t:
+  Smt (DefineConst 1320%Z (Unop (ZeroExtend 8%N) (Manyop Concat [Val (Val_Bits (BV 4%N 0x0%Z)) Mk_annot; Unop (Extract 51%N 0%N) (Val (Val_Symbolic 43%Z) Mk_annot) Mk_annot] Mk_annot) Mk_annot)) Mk_annot :t:
+  Smt (DeclareConst 1321%Z (Ty_BitVec 64%N)) Mk_annot :t:
+  ReadMem (RegVal_Base (Val_Symbolic 1321%Z)) (RegVal_Base (Val_Enum ((Mk_enum_id 6%nat), Mk_enum_ctor 0%nat))) (RegVal_Base (Val_Symbolic 1320%Z)) 8%N None Mk_annot :t:
+  Smt (DefineConst 1324%Z (Val (Val_Symbolic 1321%Z) Mk_annot)) Mk_annot :t:
+  WriteReg "R5" [] (RegVal_Base (Val_Symbolic 1324%Z)) Mk_annot :t:
+  Smt (DefineConst 1325%Z (Manyop (Bvmanyarith Bvadd) [Val (Val_Symbolic 29%Z) Mk_annot; Val (Val_Bits (BV 64%N 0x4%Z)) Mk_annot] Mk_annot)) Mk_annot :t:
+  WriteReg "_PC" [] (RegVal_Base (Val_Symbolic 1325%Z)) Mk_annot :t:
   tnil
 .
