pkvm_handler/a7428.v
@@ -2,11 +2,11 @@ From isla Require Import opsem.
 
 Definition a7428 : isla_trace :=
   Smt (DeclareConst 0%Z (Ty_BitVec 16%N)) Mk_annot :t:
-  Smt (DefineConst 150%Z (Manyop (Bvmanyarith Bvor) [Val (Val_Bits (BV 64%N 0x0%Z)) Mk_annot; Unop (ZeroExtend 48%N) (Val (Val_Symbolic 0%Z) Mk_annot) Mk_annot] Mk_annot)) Mk_annot :t:
-  WriteReg "R6" [] (RegVal_Base (Val_Symbolic 150%Z)) Mk_annot :t:
-  Smt (DeclareConst 151%Z (Ty_BitVec 64%N)) Mk_annot :t:
-  ReadReg "_PC" [] (RegVal_Base (Val_Symbolic 151%Z)) Mk_annot :t:
-  Smt (DefineConst 152%Z (Manyop (Bvmanyarith Bvadd) [Val (Val_Symbolic 151%Z) Mk_annot; Val (Val_Bits (BV 64%N 0x4%Z)) Mk_annot] Mk_annot)) Mk_annot :t:
-  WriteReg "_PC" [] (RegVal_Base (Val_Symbolic 152%Z)) Mk_annot :t:
+  Smt (DefineConst 148%Z (Manyop (Bvmanyarith Bvor) [Val (Val_Bits (BV 64%N 0x0%Z)) Mk_annot; Unop (ZeroExtend 48%N) (Val (Val_Symbolic 0%Z) Mk_annot) Mk_annot] Mk_annot)) Mk_annot :t:
+  WriteReg "R6" [] (RegVal_Base (Val_Symbolic 148%Z)) Mk_annot :t:
+  Smt (DeclareConst 149%Z (Ty_BitVec 64%N)) Mk_annot :t:
+  ReadReg "_PC" [] (RegVal_Base (Val_Symbolic 149%Z)) Mk_annot :t:
+  Smt (DefineConst 150%Z (Manyop (Bvmanyarith Bvadd) [Val (Val_Symbolic 149%Z) Mk_annot; Val (Val_Bits (BV 64%N 0x4%Z)) Mk_annot] Mk_annot)) Mk_annot :t:
+  WriteReg "_PC" [] (RegVal_Base (Val_Symbolic 150%Z)) Mk_annot :t:
   tnil
 .
